fix parser error for likesbranchedbetree

Splinter/Betree/LikesBranchedBetree.i.dfy
@@ -5,60 +5,99 @@ include "Branches.i.dfy"
 include "../Disk/GenericDisk.i.dfy"
 include "Domain.i.dfy"
 include "../../lib/Base/mathematics.i.dfy"
-include "../../lib/Buckets/BoundedPivotsLib.i.dfy"
-include "LinkedBetree.i.dfy"
+include "../../lib/Base/Multisets.i.dfy"
+// include "../../lib/Buckets/BoundedPivotsLib.i.dfy"
+include "BranchedBetree.i.dfy"
 include "SplitRequest.i.dfy"
 
 module LikesBranchedBetreeMod
 {
-  import opened BoundedPivotsLib
-  import opened DomainMod
-  import opened GenericDisk
-  import opened LSNMod
-  import opened MemtableMod
-  import opened MsgHistoryMod
-  import opened Options
+  // import opened BoundedPivotsLib
+  // import opened DomainMod
+  import GenericDisk
+  // import opened LSNMod
+  // import opened MemtableMod
+  // import opened MsgHistoryMod
+  // import opened Options
   import opened Sequences
   import opened StampedMod
-  import opened Upperbounded_Lexicographic_Byte_Order_Impl
-  import opened Upperbounded_Lexicographic_Byte_Order_Impl.Ord
-  import opened KeyType
-  import opened ValueMessage
+  // import opened Upperbounded_Lexicographic_Byte_Order_Impl
+  // import opened Upperbounded_Lexicographic_Byte_Order_Impl.Ord
+  // import opened KeyType
+  // import opened ValueMessage
   import opened Maps
-  import TotalKMMapMod
-  import opened SplitRequestMod
+  // import TotalKMMapMod
+  // import opened SplitRequestMod
+  import opened BranchesMod
+  import opened Multisets
 
   import M = Mathematics
   import BB = BranchedBetreeMod
 
   type Pointer = GenericDisk.Pointer
   type Address = GenericDisk.Address
-  type StampedBetree = Stamped<BranchedBetree>
+  type Ranking = GenericDisk.Ranking
+  type StampedBetree = Stamped<BB.BranchedBetree>
 
-  function TransitiveLikes(dv: DiskView, ptr: Pointer, r: Ranking) : Likes
+  type Likes = multiset<Address>
+
+  function NoLikes() : Likes
   {
-    if ptr.None
+    multiset{}
+  }
+
+  function mapsum<T>(s: map<T, Likes>) : Likes
+  {
+    if s.Keys == {} then NoLikes()
+    else (
+      var k :| k in s.Keys;
+      s[k] + mapsum(MapRemove1(s, k))
+    )
+  }
+
+  function toSeq<T>(s: set<T>) : seq<T> 
+  {
+    if s == {} then []
+    else (
+      var e :| e in s;
+      [e] + toSeq(s - {e})
+    )
+  }
+
+  // TODO: add to branch module
+  function BranchLikes(root: Address, branches: Branches) : Likes
+  {
+    NoLikes() 
+  }
+
+  function TransitiveLikes(bbtree: BB.BranchedBetree, r: Ranking) : Likes
+    requires bbtree.WF()
+    requires bbtree.ValidRanking(r)
+    decreases bbtree.GetRank(r)
+  {
+    if !bbtree.HasRoot()
     then
       NoLikes()
     else (
-      var node := dv.get(ptr);
-      var branchLikes = sum(fcnlmap(node.buffers,
-        bufferRoot => BranchMod.TransitiveLikes(branches, bufferRoot)));
-      var childrenLikes = sum(set(chlidren),
-        childPtr => TransitiveLikes(dv, childPtr, r));
+      var root := bbtree.Root();
+      var branchLikes := mapsum(map addr | addr in root.buffers :: BranchLikes(addr, bbtree.branches)); 
+      var childrenLikes := mapsum(map i | 0 <= i < |root.children| :: TransitiveLikes(bbtree.ChildAtIdx(i), r));
       branchLikes + childrenLikes
     )
   }
 
   function ImperativeLikes(v: Variables) : Likes
   {
-    var branchLikes := sum(fcnlmap(v.branchLikes,
-        branchRoot => BranchMod.TransitiveLikes(branches, branchRoot)) * v.branchLikes.multiplicity(branchRoot))
+    var branchLikes := mapsum(map addr | addr in v.branchLikes :: 
+      Multiply(BranchLikes(addr, v.branchedVars.branched.branches), v.branchLikes[addr]));
     branchLikes + v.betreeLikes
   }
 
-  predicate ImperativeAgreement(v: Variables) {
-    TransitiveLikes(blah, v.branchedVars.root, blah) == ImperativeLikes(v)
+  predicate ImperativeAgreement(v: Variables) 
+  {
+    && v.branchedVars.branched.Acyclic()
+    // && v.branchedVars.branched.Valid()
+    && TransitiveLikes(v.branchedVars.branched, v.branchedVars.branched.TheRanking()) == ImperativeLikes(v)
   }
 
   datatype Variables = Variables(
@@ -67,39 +106,68 @@ module LikesBranchedBetreeMod
   
     // plus imperatively-maintained view of the functional TransitiveLikes:
     betreeLikes: Likes, // internal refs
-    branchLikes: Likes, // outgoing refs
+    branchLikes: Likes // outgoing refs
   )
   {
     predicate WF() {
-      && bbtree.WF()
+      && branchedVars.WF()
+    }
+  }
+
+  datatype TransitionLabel =
+    | InternalAllocationsLabel(addrs: set<Address>)
+    | InternalLabel()   // Local No-op label
+  {
+    function I() : BB.TransitionLabel
+    {
+      match this {
+        case InternalAllocationsLabel(addrs) => BB.InternalAllocationsLabel(toSeq(addrs), [])
+        case _ => BB.InternalLabel
+      }
     }
   }
 
   predicate InternalGrow(v: Variables, v': Variables, lbl: TransitionLabel, step: Step)
   {
     && lbl.InternalAllocationsLabel?
-    // NB step.newRootAddr, allocation, and lbl are all tied together up in
-    // LinkedBetree.InternalGrow.
-    && BB.InternalGrow(v.branchedVars, v'.branchedVars, lbl.I(), step.I())
+    && BB.Next(v.branchedVars, v'.branchedVars, lbl.I())
+    // && BB.InternalGrow(v.branchedVars, v'.branchedVars, lbl.I(), step.I())
     && v' == v.(
       branchedVars := v'.branchedVars,  // admit relational update above
-      betreeLikes := v.betreeLikes,
-    )
-  }
-  
-  predicate InternalCompact(v: Variables, v': Variables, lbl: TransitionLabel, step: Step)
-  {
-    && lbl.InternalAllocationsLabel?
-    && LinkedBetreeMod.InternalCompact(v.betree, v'.betree, lbl.I(), step.I())
-    && var unlikedBranchRoots = multiset{Set(root.buffers[compactStart..compactEnd])};
-    && var unlikedBetreeNodes := step.path.AddrsOnPath();
-    && v' == v.(
-      branchedVars := v'.branchedVars,  // admit relational update above
-      betreeLikes := v.betreeLikes + lbl.treeAddrs - unlikedBetreeNodes,
-      branchLikes := v.branchLikes + multiset{step.compactedBranch.root} - unlikedBranchRoots,
+      betreeLikes := v.betreeLikes
     )
   }
 
-  
+  predicate InternalCompact(v: Variables, v': Variables, lbl: TransitionLabel, step: Step)
+  {
+    && lbl.InternalAllocationsLabel?
+    && BB.Next(v.branchedVars, v'.branchedVars, lbl.I())
+//     && LinkedBetreeMod.InternalCompact(v.betree, v'.betree, lbl.I(), step.I())
+
+    // should be in step
+    // && var root := v.branchedVars.branched.Root() 
+    // && var unlikedBranchRoots := multiset{Set(root.buffers[compactStart..compactEnd])};
+    // && var unlikedBetreeNodes := step.path.AddrsOnPath();
+
+    // && v' == v.(
+    //   branchedVars := v'.branchedVars,  // admit relational update above
+    //   betreeLikes := v.betreeLikes + step.treeAddrs - unlikedBetreeNodes,
+    //   branchLikes := v.branchLikes + multiset{step.compactedBranch.root} - unlikedBranchRoots,
+    // )
+  }
+
+  datatype Step =
+    | InternalGrow(newRootAddr: Address)
+    | InternalCompact()
+    | InternalLabel()   // Local No-op label
+  {
+  //   function I() : BB.TransitionLabel
+  //   {
+  //     match this {
+  //       case InternalAllocationsLabel(addrs) => BB.InternalAllocationsLabel(toSeq(addrs), [])
+  //       case _ => BB.InternalLabel
+  //     }
+  //   }
+  }
 
 } // module
